```agda
{-# OPTIONS --without-K --exact-split #-}

open import UF-Equiv
open import UF-FunExt
open import UF-Subsingletons
open import SpartanMLTT
open import Two-Properties hiding (zero-is-not-one)
open import NaturalsOrder
open import IntegersOrder
open import IntegersB
open import NaturalsAddition renaming (_+_ to _+â„•_)
open import IntegersAddition renaming (_+_ to _+â„¤_)
open import IntegersNegation renaming (-_  to  âˆ’â„¤_)
open import UF-Subsingletons
open import NaturalsOrder
open import DecidableAndDetachable

module BelowAndAbove (fe : FunExt)where

open import TernaryBoehmRealsPrelude fe

```

downLeft, downMid and downRight

```
downLeft downMid downRight : â„¤ â†’ â„¤
downLeft  a = a +â„¤ a
downMid   a = succâ„¤ (downLeft a)
downRight a = succâ„¤ (downMid  a)
```

below and below'

```
_below_ : â„¤ â†’ â„¤ â†’ ğ“¤â‚€ Ì‡ 
a below b = downLeft b â‰¤â„¤ a â‰¤â„¤ downRight b

downLeft-below  : (a : â„¤) â†’ downLeft a below a
downLeft-below  a = (0 , refl) , (2 , refl)

downMid-below   : (a : â„¤) â†’ downMid a below a
downMid-below   a = (1 , refl) , (1 , refl)

downRight-below : (a : â„¤) â†’ downRight a below a
downRight-below a = (2 , refl) , (0 , refl)

_below'_ : â„¤ â†’ â„¤ â†’ ğ“¤â‚€ Ì‡
a below' b = (a â‰¡ downLeft b) + (a â‰¡ downMid b) + (a â‰¡ downRight b)

below'-implies-below : (a b : â„¤) â†’ a below' b â†’ a below b
below'-implies-below .(downLeft  b) b (inl      refl ) = downLeft-below b
below'-implies-below .(downMid   b) b (inr (inl refl)) = downMid-below b
below'-implies-below .(downRight b) b (inr (inr refl)) = downRight-below b

below-implies-below' : (a b : â„¤) â†’ a below b â†’ a below' b
below-implies-below' a b ((0 , e) , _)
 = inl (e â»Â¹)
below-implies-below' a b ((1 , e) , _)
 = (inr âˆ˜ inl) (e â»Â¹)
below-implies-below' a b ((2 , e) , _)
 = (inr âˆ˜ inr) (e â»Â¹)
below-implies-below' a b ((succ (succ (succ _)) , _) , (0 , f))
 = (inr âˆ˜ inr) f
below-implies-below' a b ((succ (succ (succ _)) , _) , (1 , f))
 = (inr âˆ˜ inl) (succâ„¤-lc f)
below-implies-below' a b ((succ (succ (succ _)) , _) , (2 , f))
 = inl (succâ„¤-lc (succâ„¤-lc f))
below-implies-below' a b ((succ (succ (succ n)) , e) , (succ (succ (succ m)) , f))
 = ğŸ˜-elim (kâ‰¢2 kâ‰¡2)
 where   
   k : â„•
   k = (succ (succ (succ (succ (succ (succ (n +â„• m)))))))
   Î· : downLeft b +pos k â‰¡ downRight b
   Î· = (ap ((succâ„¤ ^ 6) âˆ˜ downLeft b +â„¤_) (pos-addition-equiv-to-â„• n m â»Â¹)
     âˆ™ ap (succâ„¤ ^ 6) (â„¤+-assoc (downLeft b) (pos n) (pos m) â»Â¹)
     âˆ™ ap (succâ„¤ ^ 5) (â„¤-left-succ-pos (downLeft b +pos n) m â»Â¹)
     âˆ™ ap (succâ„¤ ^ 4) (â„¤-left-succ-pos (succâ„¤ (downLeft b +pos n)) m â»Â¹)
     âˆ™ ap (succâ„¤ ^ 3) (â„¤-left-succ-pos ((succâ„¤ ^ 2) (downLeft b +pos n)) m â»Â¹)
     âˆ™ ap ((succâ„¤ ^ 3) âˆ˜ (_+pos m)) e
     âˆ™ f)
   Î¶ : downLeft b +pos 2 â‰¡ downRight b
   Î¶ = refl
   kâ‰¡2 : k â‰¡ 2
   kâ‰¡2 = pos-lc k 2 (â„¤+-lc (pos k) (pos 2) (downLeft b) (Î· âˆ™ Î¶ â»Â¹))
   kâ‰¢2 : k â‰¢ 2
   kâ‰¢2 = Î» ()
```

upLeft and upRight

```
upRight : â„¤ â†’ â„¤
upRight x = sign x (num x /2)

upLeft' : (x : â„¤) â†’ even x + odd x â†’ â„¤
upLeft' x (inl _) = predâ„¤ (upRight x)
upLeft' x (inr _) =        upRight x

upLeft : â„¤ â†’ â„¤
upLeft x = upLeft' x (even-or-odd? x)
```

upLeft elimination

```
upLeft-elim : (x : â„¤) â†’ (P : â„¤ â†’ ğ“¤ Ì‡ )
            â†’ P (predâ„¤ (upRight x)) â†’ P (upRight x)
            â†’ P (upLeft x)
upLeft-elim x P Pe Po with even-or-odd? x
... | (inl e) = Pe
... | (inr o) = Po

upLeftÂ²-elim : (x : â„¤) â†’ (P : â„¤ â†’ â„¤ â†’ ğ“¤ Ì‡ )
             â†’ P (predâ„¤ (upRight x)) (predâ„¤ (upRight (succâ„¤ (succâ„¤ x))))
             â†’ P (upRight x) (upRight (succâ„¤ (succâ„¤ x)))
             â†’ P (upLeft x) (upLeft (succâ„¤ (succâ„¤ x)))
upLeftÂ²-elim x P Pe Po with even-or-odd? x
... | (inl e) = transport (P (predâ„¤ (upRight x)))
                  (ap (upLeft' (succâ„¤ (succâ„¤ x)))
                     (even-or-odd-is-prop (succâ„¤ (succâ„¤ x))
                       (inl (even-succ-succ x e))
                       (even-or-odd? (succâ„¤ (succâ„¤ x)))))
                  Pe
... | (inr o) = transport (P (upRight x))
                  (ap (upLeft' (succâ„¤ (succâ„¤ x)))
                     (even-or-odd-is-prop (succâ„¤ (succâ„¤ x))
                        (inr (odd-succ-succ x o))
                        (even-or-odd? (succâ„¤ (succâ„¤ x)))))
                  Po

upLeftÂ²-elim-pred : (x : â„¤) â†’ (P : â„¤ â†’ â„¤ â†’ ğ“¤ Ì‡ )
                  â†’ P (predâ„¤ (upRight (predâ„¤ (predâ„¤ x)))) (predâ„¤ (upRight x))
                  â†’ P (upRight (predâ„¤ (predâ„¤ x))) (upRight x)
                  â†’ P (upLeft (predâ„¤ (predâ„¤ x))) (upLeft x)
upLeftÂ²-elim-pred x P Pe Po
 = transport (P (upLeft y))
     (ap upLeft (ap succâ„¤ (succpredâ„¤ (predâ„¤ x)) âˆ™ succpredâ„¤ x))
     Py
 where
   y : â„¤
   y = predâ„¤ (predâ„¤ x)
   Pe' : P (predâ„¤ (upRight y)) (predâ„¤ (upRight (succâ„¤ (succâ„¤ y))))
   Pe' = transport
           (Î» - â†’ P (predâ„¤ (upRight (predâ„¤ (predâ„¤ x)))) (predâ„¤ (upRight -)))
           (succpredâ„¤ _ â»Â¹ âˆ™ ap succâ„¤ (succpredâ„¤ _ â»Â¹))
           Pe
   Po' : P (upRight y) (upRight (succâ„¤ (succâ„¤ y)))
   Po' = transport
           (Î» - â†’ P (upRight (predâ„¤ (predâ„¤ x))) (upRight -))
           (succpredâ„¤ _ â»Â¹ âˆ™ ap succâ„¤ (succpredâ„¤ _ â»Â¹))
           Po
   Py : P (upLeft (predâ„¤ (predâ„¤ x))) (upLeft (succâ„¤ (succâ„¤ (predâ„¤ (predâ„¤ x)))))
   Py = upLeftÂ²-elim y P Pe' Po'
```

above and above'

```
_above_ : â„¤ â†’ â„¤ â†’ ğ“¤â‚€ Ì‡ 
b above a = upLeft a â‰¤â„¤ b â‰¤â„¤ upRight a

_above'_ : â„¤ â†’ â„¤ â†’ ğ“¤â‚€ Ì‡
a above' b = (a â‰¡ upLeft b) + (a â‰¡ upRight b)

upLeft-â‰¡-+ : (a : â„¤) â†’ (upLeft a â‰¡ upRight a) + (succâ„¤ (upLeft a) â‰¡ upRight a)
upLeft-â‰¡-+ a = upLeft-elim a (Î» - â†’ (- â‰¡ upRight a) + (succâ„¤ - â‰¡ upRight a))
                 (inr (succpredâ„¤ _)) (inl refl)

upLeftâ‰¤upRight : (a : â„¤) â†’ upLeft a â‰¤â„¤ upRight a
upLeftâ‰¤upRight a = Cases (upLeft-â‰¡-+ a) (0 ,_) (1 ,_)

upLeft-above : (a : â„¤) â†’ upLeft a above a
upLeft-above a = (0 , refl) , upLeftâ‰¤upRight a

upRight-above : (a : â„¤) â†’ upRight a above a
upRight-above a = (upLeftâ‰¤upRight a) , (0 , refl)

above'-implies-above : (a b : â„¤) â†’ a above' b â†’ a above b
above'-implies-above .(upLeft  b) b (inl refl) = upLeft-above b
above'-implies-above .(upRight b) b (inr refl) = upRight-above b

a<bâ†’aâ‰¢b : âˆ€ a b â†’ (b <â„¤ a) â†’ a â‰¢ b
a<bâ†’aâ‰¢b a a (n , a<a) refl = Î³ Î³'
 where
   Î³' : 0 â‰¡ succ n
   Î³' = pos-lc _ _ (â„¤+-lc _ _ a (a<a â»Â¹ âˆ™ â„¤-left-succ-pos a n))
   Î³ : 0 â‰¢ succ n
   Î³ ()

impossible : (a b : â„¤) â†’ (pos 2) â‰¤â„¤ b â†’ upLeft a +â„¤ b â‰¢ upRight a
impossible a .(pos 2 +â„¤ (pos n)) (n , refl) e
 = Cases (upLeft-â‰¡-+ a)
     (Î» g â†’ a<bâ†’aâ‰¢b (pos 2 +pos n) (pos 0) (1 +â„• n , Î³   )
       (â„¤+-lc (pos 2 +pos n) (pos 0) (upLeft a) (e âˆ™ g â»Â¹)))
     (Î» g â†’ a<bâ†’aâ‰¢b (pos 2 +pos n) (pos 1) (     n , refl)
       (â„¤+-lc (pos 2 +pos n) (pos 1) (upLeft a) (e âˆ™ g â»Â¹)))
 where
   Î³ : succâ„¤ (pos 0) +â„¤ pos (1 +â„• n) â‰¡ (pos 2 +pos n)
   Î³ = ap (pos 1 +â„¤_) (pos-addition-equiv-to-â„• 1 n â»Â¹)
     âˆ™ â„¤+-assoc (pos 1) (pos 1) (pos n) â»Â¹

above-implies-above' : (a b : â„¤) â†’ a above b â†’ a above' b
above-implies-above' a b ((0 , refl) , (m , f)) = inl refl
above-implies-above' a b ((succ n , e) , zero , refl) = inr refl
above-implies-above' a b ((1 , e) , succ m , f)
 = Cases (upLeft-â‰¡-+ b) (Î» g â†’ ğŸ˜-elim Î·)
                        (Î» g â†’ inr (e â»Â¹ âˆ™ g))
 where
   Î¶ : pos 2 +â„¤ pos m â‰¡ succâ„¤ (succâ„¤ (pos m))
   Î¶ = pos-addition-equiv-to-â„• 2 m
     âˆ™ ap pos (addition-commutativity 2 m)
   Î³ : upLeft b +â„¤ succâ„¤ (succâ„¤ (pos m)) â‰¡ upRight b
   Î³ = ap succâ„¤ (â„¤-left-succ-pos (upLeft b) m â»Â¹)
     âˆ™ ap (Î» - â†’ succâ„¤ (- +pos m)) e
     âˆ™ f
   Î· = impossible b (succâ„¤ (succâ„¤ (pos m))) (m , Î¶) Î³
above-implies-above' a b ((succ (succ n) , e) , succ m , f)
 = ğŸ˜-elim (impossible b (pos (succ (succ (succ n))) +pos m)
             (succ n +â„• m , Î¶) Î³)
 where
   Î³ : upLeft b +â„¤ (pos (succ (succ (succ n))) +pos m) â‰¡ upRight b
   Î³ = â„¤+-assoc (upLeft b) (pos (succ (succ (succ n)))) (pos m) â»Â¹
     âˆ™ â„¤-left-succ-pos _ m
     âˆ™ ap (Î» - â†’ succâ„¤ (- +pos m)) e
     âˆ™ f
   Î¶ : pos 2 +pos (succ n +â„• m) â‰¡ pos (succ (succ (succ n))) +pos m
   Î¶ = ap (pos 2 +â„¤_) (pos-addition-equiv-to-â„• (succ n) m â»Â¹)
     âˆ™ â„¤+-assoc (pos 2) (pos (succ n)) (pos m) â»Â¹
     âˆ™ ap (_+pos m)
         (ap succâ„¤ (pos-addition-equiv-to-â„• 2 n)
       âˆ™ ap (pos âˆ˜ succ) (addition-commutativity 2 n))
```

Relationship between below and above

```
upRight-suc : (a : â„¤) â†’ upRight (succâ„¤ (succâ„¤ a)) â‰¡ succâ„¤ (upRight a)
upRight-suc (pos zero) = refl
upRight-suc (pos (succ zero)) = refl
upRight-suc (pos (succ (succ x))) = refl
upRight-suc (negsucc zero) = refl
upRight-suc (negsucc (succ zero)) = refl
upRight-suc (negsucc (succ (succ x))) = refl

pred-upRight-suc : (a : â„¤) â†’ predâ„¤ (upRight (succâ„¤ (succâ„¤ a))) â‰¡ succâ„¤ (predâ„¤ (upRight a))
pred-upRight-suc (pos zero) = refl
pred-upRight-suc (pos (succ zero)) = refl
pred-upRight-suc (pos (succ (succ x))) = refl
pred-upRight-suc (negsucc zero) = refl
pred-upRight-suc (negsucc (succ zero)) = refl
pred-upRight-suc (negsucc (succ (succ x))) = refl

upLeft-suc : (a : â„¤) â†’ upLeft (succâ„¤ (succâ„¤ a)) â‰¡ succâ„¤ (upLeft a)
upLeft-suc a
 = upLeftÂ²-elim a (Î» a b â†’ b â‰¡ succâ„¤ a) (pred-upRight-suc a) (upRight-suc a)

pred-upRight-pred : (a : â„¤) â†’ predâ„¤ (upRight (predâ„¤ (predâ„¤ a))) â‰¡ predâ„¤ (predâ„¤ (upRight a))
pred-upRight-pred (pos zero) = refl
pred-upRight-pred (pos (succ zero)) = refl
pred-upRight-pred (pos (succ (succ x))) = refl
pred-upRight-pred (negsucc zero) = refl
pred-upRight-pred (negsucc (succ zero)) = refl
pred-upRight-pred (negsucc (succ (succ x))) = refl

upRight-pred : (a : â„¤) â†’ upRight (predâ„¤ (predâ„¤ a)) â‰¡ predâ„¤ (upRight a)
upRight-pred (pos 0) = refl
upRight-pred (pos 1) = refl
upRight-pred (pos (succ (succ x))) = refl
upRight-pred (negsucc 0) = refl
upRight-pred (negsucc 1) = refl
upRight-pred (negsucc (succ (succ x))) = refl

upLeft-pred : (a : â„¤) â†’ upLeft (predâ„¤ (predâ„¤ a)) â‰¡ predâ„¤ (upLeft a)
upLeft-pred a
 = upLeftÂ²-elim-pred a (Î» a b â†’ a â‰¡ predâ„¤ b) (pred-upRight-pred a) (upRight-pred a)

â„¤-elim : (P : â„¤ â†’ ğ“¤ Ì‡ )
       â†’ ((n : â„•) â†’ P (pos n)) â†’ ((n : â„•) â†’ P (negsucc n))
       â†’ Î  P
â„¤-elim P Pp Pn (pos     n) = Pp n
â„¤-elim P Pp Pn (negsucc n) = Pn n

upLeft-downLeft-pos : (b : â„•) â†’ succâ„¤ (upLeft (downLeft (pos b))) â‰¡ pos b
upLeft-downLeft-pos 0 = refl
upLeft-downLeft-pos (succ b)
 = ap (succâ„¤ âˆ˜ upLeft âˆ˜ succâ„¤) (â„¤-left-succ-pos (pos b) b)
 âˆ™ ap succâ„¤ (upLeft-suc (downLeft (pos b)))
 âˆ™ ap succâ„¤ (upLeft-downLeft-pos b)

upLeft-downLeft-negsucc : (b : â„•) â†’ succâ„¤ (upLeft (downLeft (negsucc b))) â‰¡ negsucc b
upLeft-downLeft-negsucc 0 = refl
upLeft-downLeft-negsucc (succ b)
 = ap (succâ„¤ âˆ˜ upLeft âˆ˜ predâ„¤) (â„¤-left-pred-negsucc (negsucc b) b)
 âˆ™ ap succâ„¤ (upLeft-pred (downLeft (negsucc b)))
 âˆ™ succpredâ„¤ _ âˆ™ predsuccâ„¤ _ â»Â¹
 âˆ™ ap predâ„¤ (upLeft-downLeft-negsucc b)

upRight-downLeft-pos : (b : â„•) â†’ pos b â‰¡ upRight (downLeft (pos b))
upRight-downLeft-pos 0 = refl
upRight-downLeft-pos (succ b)
 = ap succâ„¤ (upRight-downLeft-pos b)
 âˆ™ upRight-suc (downLeft (pos b)) â»Â¹
 âˆ™ ap (upRight âˆ˜ succâ„¤) (â„¤-left-succ-pos (pos b) b â»Â¹)

upRight-downLeft-negsucc : (b : â„•) â†’ negsucc b â‰¡ upRight (downLeft (negsucc b))
upRight-downLeft-negsucc 0 = refl
upRight-downLeft-negsucc (succ b)
 = ap predâ„¤ (upRight-downLeft-negsucc b)
 âˆ™ upRight-pred (downLeft (negsucc b)) â»Â¹
 âˆ™ ap (upRight âˆ˜ predâ„¤) (â„¤-left-pred-negsucc (negsucc b) b â»Â¹)

below-implies-above-dL : (b : â„¤) â†’ b above (downLeft b)
below-implies-above-dL b
 = (1 , â„¤-elim (Î» b â†’ succâ„¤ (upLeft (downLeft b)) â‰¡ b)
          upLeft-downLeft-pos upLeft-downLeft-negsucc b)
 , (0 , â„¤-elim (Î» b â†’ b â‰¡ upRight (downLeft b))
          upRight-downLeft-pos upRight-downLeft-negsucc b)

upLeft-downMid-pos : (b : â„•) â†’ upLeft (downMid (pos b)) â‰¡ pos b
upLeft-downMid-pos 0 = refl
upLeft-downMid-pos (succ b)
 = ap (upLeft âˆ˜ succâ„¤) (â„¤-left-succ-pos (pos b) (succ b))
 âˆ™ upLeft-suc (downMid (pos b))
 âˆ™ ap succâ„¤ (upLeft-downMid-pos b)

upLeft-downMid-negsucc : (b : â„•) â†’ upLeft (downMid (negsucc b)) â‰¡ negsucc b
upLeft-downMid-negsucc 0 = refl
upLeft-downMid-negsucc (succ b)
 = ap (upLeft âˆ˜ succâ„¤) (â„¤-left-pred-negsucc (negsucc b) (succ b))
 âˆ™ ap upLeft (succpredâ„¤ (predâ„¤ (downLeft (negsucc b))))
 âˆ™ ap (upLeft âˆ˜ predâ„¤) (predsuccâ„¤ (downLeft (negsucc b)) â»Â¹)
 âˆ™ upLeft-pred (downMid (negsucc b))
 âˆ™ ap predâ„¤ (upLeft-downMid-negsucc b)

upRight-downMid-pos : (b : â„•) â†’ pos b â‰¡ upRight (downMid (pos b))
upRight-downMid-pos 0 = refl
upRight-downMid-pos (succ b)
 = ap succâ„¤ (upRight-downMid-pos b)
 âˆ™ upRight-suc (downMid (pos b)) â»Â¹
 âˆ™ ap (upRight âˆ˜ succâ„¤ âˆ˜ succâ„¤) (â„¤-left-succ-pos (pos b) b â»Â¹)

upRight-downMid-negsucc : (b : â„•) â†’ negsucc b â‰¡ upRight (downMid (negsucc b))
upRight-downMid-negsucc 0 = refl
upRight-downMid-negsucc (succ b)
 = ap predâ„¤ (upRight-downMid-negsucc b)
 âˆ™ upRight-pred (downMid (negsucc b)) â»Â¹
 âˆ™ ap (upRight âˆ˜ predâ„¤) (predsuccâ„¤ _)
 âˆ™ ap upRight (â„¤-left-pred-negsucc (negsucc b) b â»Â¹)
 âˆ™ ap upRight (succpredâ„¤ _ â»Â¹)

below-implies-above-dM : (b : â„¤) â†’ b above (downMid b)
below-implies-above-dM b
 = (0 , â„¤-elim (Î» b â†’ upLeft (downMid b) â‰¡ b)
          upLeft-downMid-pos upLeft-downMid-negsucc b)
 , (0 , â„¤-elim (Î» b â†’ b â‰¡ upRight (downMid b))
          upRight-downMid-pos upRight-downMid-negsucc b)

upLeft-downRight-pos : (b : â„•) â†’ upLeft (downRight (pos b)) â‰¡ pos b
upLeft-downRight-pos 0 = refl
upLeft-downRight-pos (succ b)
 = ap (upLeft âˆ˜ succâ„¤) (â„¤-left-succ-pos (pos b) (succ (succ b)))
 âˆ™ upLeft-suc (downRight (pos b))
 âˆ™ ap succâ„¤ (upLeft-downRight-pos b)

upLeft-downRight-negsucc : (b : â„•) â†’ upLeft (downRight (negsucc b)) â‰¡ negsucc b
upLeft-downRight-negsucc 0 = refl
upLeft-downRight-negsucc (succ b)
 = ap (upLeft âˆ˜ succâ„¤ âˆ˜ succâ„¤) (â„¤-left-pred-negsucc (negsucc b) (succ b))
 âˆ™ ap (upLeft âˆ˜ succâ„¤) (succpredâ„¤ (predâ„¤ (downLeft (negsucc b))))
 âˆ™ ap upLeft (succpredâ„¤ (downLeft (negsucc b)))
 âˆ™ ap upLeft (predsuccâ„¤ (downLeft (negsucc b))) â»Â¹
 âˆ™ ap (upLeft âˆ˜ predâ„¤) (predsuccâ„¤ (succâ„¤ (downLeft (negsucc b))) â»Â¹)
 âˆ™ upLeft-pred (downRight (negsucc b))
 âˆ™ ap predâ„¤ (upLeft-downRight-negsucc b)

upRight-downRight-pos : (b : â„•) â†’ succâ„¤ (pos b) â‰¡ upRight (downRight (pos b))
upRight-downRight-pos 0 = refl
upRight-downRight-pos (succ b)
 = ap succâ„¤ (upRight-downRight-pos b)
 âˆ™ upRight-suc (downRight (pos b)) â»Â¹
 âˆ™ ap (upRight âˆ˜ succâ„¤ âˆ˜ succâ„¤ âˆ˜ succâ„¤) (â„¤-left-succ-pos (pos b) b â»Â¹)

upRight-downRight-negsucc : (b : â„•) â†’ succâ„¤ (negsucc b) â‰¡ upRight (downRight (negsucc b))
upRight-downRight-negsucc 0 = refl
upRight-downRight-negsucc (succ b)
 = upRight-downLeft-negsucc b
 âˆ™ ap upRight (succpredâ„¤ _ â»Â¹)
 âˆ™ ap (upRight âˆ˜ succâ„¤) (â„¤-left-pred-negsucc (negsucc b) b â»Â¹)
 âˆ™ ap (upRight âˆ˜ succâ„¤) (succpredâ„¤ _ â»Â¹)

below-implies-above-dR : (b : â„¤) â†’ b above (downRight b)
below-implies-above-dR b
 = (0 , â„¤-elim (Î» b â†’ upLeft (downRight b) â‰¡ b)
           upLeft-downRight-pos upLeft-downRight-negsucc b)
 , (1 , â„¤-elim (Î» b â†’ succâ„¤ b â‰¡ upRight (downRight b))
           upRight-downRight-pos upRight-downRight-negsucc b)

below'-implies-above : (a b : â„¤) â†’ a below' b â†’ b above a
below'-implies-above .(downLeft  b) b (inl refl)
 = below-implies-above-dL b
below'-implies-above .(downMid   b) b (inr (inl refl))
 = below-implies-above-dM b
below'-implies-above .(downRight b) b (inr (inr refl))
 = below-implies-above-dR b

above'-implies-below : (a b : â„¤) â†’ a above' b â†’ b below a
above'-implies-below .(upLeft b) b (inl refl) = {!!}
above'-implies-below a b (inr x) = {!!}

below-implies-above : (a b : â„¤) â†’ a below b â†’ b above a
below-implies-above a b = (below'-implies-above a b) âˆ˜ (below-implies-below' a b)

above-downLeft : (a : â„¤) â†’ a above (downLeft a)
above-downLeft a = below-implies-above (downLeft a) a (downLeft-below a)

above-downMid : (a : â„¤) â†’ a above (downMid a)
above-downMid a = below-implies-above (downMid a) a (downMid-below a)

above-downRight : (a : â„¤) â†’ a above (downRight a)
above-downRight a = below-implies-above (downRight a) a (downRight-below a)
```

Recursive above

```

data Vec (X : ğ“¤ Ì‡ ) : â„• â†’ ğ“¤ Ì‡ where
  [] : Vec X 0
  _::_ : {n : â„•} â†’ X â†’ Vec X n â†’ Vec X (succ n)

get : {X : ğ“¤ Ì‡ } {n : â„•} â†’ Vec X n â†’ (i : â„•) â†’ i <â„• n â†’ X
get (x :: vs) zero i<n = x
get (x :: vs) (succ i) i<n = get vs i i<n

somewhere-above : â„¤ â†’ â„¤ â†’ ğ“¤â‚€ Ì‡ 
somewhere-above a b = Î£ (n , ls , _) ê‰ (Î£ (Vec â„¤))
                    , ((i : â„•) (i<n : i <â„• n)
                    â†’ get {!!} {!!} {!!} above get ls {!!} {!//!}) 
