```agda
{-# OPTIONS --without-K --exact-split #-}

open import SpartanMLTT hiding (decidable)
open import Two-Properties hiding (zero-is-not-one)
open import NaturalsOrder
open import NaturalsAddition renaming (_+_ to _+â„•_)
open import IntegersB
-- open import IntegersOrder
open import IntegersAddition renaming (_+_ to _+â„¤_)
open import IntegersNegation renaming (-_  to  âˆ’â„¤_)
open import UF-Subsingletons

module BoehmReals (fe : {ğ“¤ ğ“¥ : Universe} â†’ {X : ğ“¤ Ì‡ } {Y : X â†’ ğ“¥ Ì‡ } {f g : Î  Y}
                           â†’ f âˆ¼ g â†’ f â‰¡ g) where

open import InfiniteSearch2 fe

{-# BUILTIN INTEGER       â„¤       #-}
{-# BUILTIN INTEGERPOS    pos     #-}
{-# BUILTIN INTEGERNEGSUC negsucc #-}
```

â„¤ operations

```agda
Î¹ : â„• â†’ â„¤
Î¹ = pos

_â‰¤â„¤_ : â„¤ â†’ â„¤ â†’ ğ“¤â‚€ Ì‡
pos x     â‰¤â„¤ pos y     = x â‰¤â„• y
negsucc x â‰¤â„¤ negsucc y = y â‰¤â„• x
pos _     â‰¤â„¤ negsucc _ = ğŸ˜
negsucc _ â‰¤â„¤ pos _     = ğŸ™

_â‰¤â„¤_â‰¤â„¤_ : â„¤ â†’ â„¤ â†’ â„¤ â†’ ğ“¤â‚€ Ì‡ 
x â‰¤â„¤ y â‰¤â„¤ z = (x â‰¤â„¤ y) Ã— (y â‰¤â„¤ z)

_âˆ’â„¤_ : â„¤ â†’ â„¤ â†’ â„¤
x âˆ’â„¤ y = x +â„¤ (âˆ’â„¤ y)

neg-flip : (x y : â„¤) â†’ (x âˆ’â„¤ y) â‰¡ âˆ’â„¤ (y âˆ’â„¤ x)
neg-flip x y
 = ap (_âˆ’â„¤ y) (minus-minus-is-plus x â»Â¹)
 âˆ™ negation-dist (âˆ’â„¤ x) y
 âˆ™ ap (Î» - â†’ âˆ’â„¤ -) (â„¤+-comm (âˆ’â„¤ x) y)

neg-some : (x y : â„¤) â†’ (âˆ’â„¤ x) +â„¤ (âˆ’â„¤ y) â‰¡ âˆ’â„¤ (x +â„¤ y)
neg-some = negation-dist

neg-same : (x : â„¤) â†’ (x âˆ’â„¤ x) â‰¡ Î¹ 0
neg-same x = â„¤-sum-of-inverse-is-zero x

abs : â„¤ â†’ â„•
abs (pos x)     = x
abs (negsucc x) = succ x

abs-0-is-0 : abs (Î¹ 0) â‰¡ 0
abs-0-is-0 = refl

abs-neg : (x : â„¤) â†’ abs x â‰¡ abs (âˆ’â„¤ x)
abs-neg (pos 0) = refl
abs-neg (pos (succ x)) = refl
abs-neg (negsucc x) = refl

diff : â„¤ â†’ â„¤ â†’ â„•
diff x y = abs (x âˆ’â„¤ y)

abs-flip : (x y : â„¤) â†’ diff x y â‰¡ diff y x
abs-flip x y = ap abs (neg-flip x y) âˆ™ abs-neg (y âˆ’â„¤ x) â»Â¹
```

Definition of below and thus ğ•‚

```agda
_/2 : â„• â†’ â„•
0 /2 = 0
1 /2 = 0
succ (succ n) /2 = succ (n /2)

sign : â„¤ â†’ (â„• â†’ â„¤)
sign (pos     _) = pos
sign (negsucc _) = negsucc

num : â„¤ â†’ â„•
num  (pos     n) = n
num  (negsucc n) = n

odd even : â„¤ â†’ ğ“¤â‚€ Ì‡
odd (pos                   0) = ğŸ˜
odd (pos                   1) = ğŸ™
odd (pos (succ (succ x)))     = odd (pos x)
odd (negsucc               0) = ğŸ™
odd (negsucc               1) = ğŸ˜
odd (negsucc (succ (succ x))) = odd (negsucc x)
even x = Â¬ odd x

even-or-odd? : (x : â„¤) â†’ even x + odd x
even-or-odd? (pos                   0) = inl (Î» x â†’ x)
even-or-odd? (pos                   1) = inr â‹†
even-or-odd? (pos (succ (succ x)))     = even-or-odd? (pos x)
even-or-odd? (negsucc               0) = inr â‹†
even-or-odd? (negsucc               1) = inl (Î» x â†’ x)
even-or-odd? (negsucc (succ (succ x))) = even-or-odd? (negsucc x)

odd-is-prop : (x : â„¤) â†’ is-prop (odd x)
odd-is-prop (pos                   0) = ğŸ˜-is-prop
odd-is-prop (pos                   1) = ğŸ™-is-prop
odd-is-prop (pos (succ (succ x)))     = odd-is-prop (pos x)
odd-is-prop (negsucc               0) = ğŸ™-is-prop
odd-is-prop (negsucc               1) = ğŸ˜-is-prop
odd-is-prop (negsucc (succ (succ x))) = odd-is-prop (negsucc x)

Â¬-is-prop : {X : ğ“¤ Ì‡ } â†’ is-prop (Â¬ X)
Â¬-is-prop p q = fe (Î» i â†’ ğŸ˜-is-prop (p i) (q i))

even-is-prop : (x : â„¤) â†’ is-prop (even x)
even-is-prop x = Â¬-is-prop

even-or-odd-is-prop : (x : â„¤) â†’ (p q : even x + odd x) â†’ p â‰¡ q
even-or-odd-is-prop x = +-is-prop (even-is-prop x) (odd-is-prop x) id

downLeft downMid downRight upLeft upRight : â„¤ â†’ â„¤
downLeft  x = x +â„¤ x
downMid   x = downLeft x +â„¤ (Î¹ 1)
downRight x = downLeft x +â„¤ (Î¹ 2)
upRight   x = sign x (num x /2)

upLeft' : (x : â„¤) â†’ even x + odd x â†’ â„¤
upLeft' x (inl _) = predâ„¤ (upRight x)
upLeft' x (inr _) = upRight x

upLeft    x = upLeft' x (even-or-odd? x)

odd-succ2 : (x : â„¤) â†’ odd x â†’ odd (succâ„¤ (succâ„¤ x))
odd-succ2 (pos (succ x)) o = o
odd-succ2 (negsucc 0) o = â‹†
odd-succ2 (negsucc (succ (succ x))) o = o

even-succ2 : (x : â„¤) â†’ even x â†’ even (succâ„¤ (succâ„¤ x))
even-succ2 (pos 0) e = id
even-succ2 (pos (succ x)) e = e
even-succ2 (negsucc 0) e = Î» _ â†’ e â‹†
even-succ2 (negsucc (succ zero)) e = Î» z â†’ z
even-succ2 (negsucc (succ (succ x))) e = e

upLeft-even : (x : â„¤) â†’ even x â†’ upLeft x â‰¡ predâ„¤ (upRight x)
upLeft-even x e = ap (upLeft' x) (even-or-odd-is-prop x (even-or-odd? x) (inl e))

upLeft-odd : (x : â„¤) â†’ odd x â†’ upLeft x â‰¡ upRight x
upLeft-odd x o = ap (upLeft' x) (even-or-odd-is-prop x (even-or-odd? x) (inr o))

_below_ : â„¤ â†’ â„¤ â†’ ğ“¤â‚€ Ì‡ 
x below y = downLeft y â‰¤â„¤ x â‰¤â„¤ downRight y

_below2_ : â„¤ â†’ â„¤ â†’ ğ“¤â‚€ Ì‡ 
x below2 y = downLeft (downLeft y) â‰¤â„¤ x â‰¤â„¤ downRight (downRight y)

_below'_ : â„¤ â†’ â„¤ â†’ ğ“¤â‚€ Ì‡
x below' y = (x â‰¡ downLeft y) + (x â‰¡ downMid y) + (x â‰¡ downRight y)

_below''_ : â„¤ â†’ â„¤ â†’ ğ“¤â‚€ Ì‡ 
x below'' y = diff x (downLeft y) â‰¤â„• 2

succ-lc : (x y : â„•) â†’ succ x â‰¡ succ y â†’ x â‰¡ y
succ-lc zero zero refl = refl
succ-lc (succ x) (succ .x) refl = refl

â„•-is-discrete : is-discrete â„•
â„•-is-discrete zero zero = inl refl
â„•-is-discrete zero (succ y) = inr (Î» ())
â„•-is-discrete (succ x) zero = inr (Î» ())
â„•-is-discrete (succ x) (succ y)
 = Cases (â„•-is-discrete x y) (inl âˆ˜ ap succ) (inr âˆ˜ (Î» f e â†’ f (succ-lc x y e)))

pos-lc : (x y : â„•) â†’ pos x â‰¡ pos y â†’ x â‰¡ y
pos-lc x .x refl = refl

negsucc-lc : (x y : â„•) â†’ negsucc x â‰¡ negsucc y â†’ x â‰¡ y
negsucc-lc x .x refl = refl

â„¤-is-discrete : is-discrete â„¤
â„¤-is-discrete (pos x) (pos y)
 = Cases (â„•-is-discrete x y) (inl âˆ˜ ap pos) (inr âˆ˜ (Î» f e â†’ f (pos-lc x y e)))
â„¤-is-discrete (negsucc x) (negsucc y)
 = Cases (â„•-is-discrete x y) (inl âˆ˜ ap negsucc) (inr âˆ˜ (Î» f e â†’ f (negsucc-lc x y e)))
â„¤-is-discrete (pos x) (negsucc y) = inr (Î» ())
â„¤-is-discrete (negsucc x) (pos y) = inr (Î» ())

â‰¤â„•-up : (x y : â„•) â†’ x â‰¤â„• y â†’ Â¬ (x â‰¡ y) â†’ succ x â‰¤â„• y
â‰¤â„•-up zero zero p f = f refl
â‰¤â„•-up zero (succ y) p f = â‹†
â‰¤â„•-up (succ x) (succ y) p f = â‰¤â„•-up x y p (f âˆ˜ ap succ)

â‰¤â„¤-up : (x y : â„¤) â†’ x â‰¤â„¤ y â†’ Â¬ (x â‰¡ y) â†’ succâ„¤ x â‰¤â„¤ y
â‰¤â„¤-up (pos x) (pos y) p f = â‰¤â„•-up x y p (f âˆ˜ ap pos)
â‰¤â„¤-up (negsucc 0) (pos y) _ _ = â‹†
â‰¤â„¤-up (negsucc (succ x)) (pos y) _ _ = â‹†
â‰¤â„¤-up (negsucc 0) (negsucc y) p f = f (ap negsucc (zero-minimal'' y p â»Â¹))
â‰¤â„¤-up (negsucc (succ x)) (negsucc y) p f
 = â‰¤â„•-up y (succ x) p (Î» yâ‰¡sx â†’ f (ap negsucc (yâ‰¡sx â»Â¹)))

â‰¤â„¤-split : (x y : â„¤) â†’ x â‰¤â„¤ y â†’ (x â‰¡ y) + (succâ„¤ x â‰¤â„¤ y)
â‰¤â„¤-split x y p
 = Cases (â„¤-is-discrete x y) inl (inr âˆ˜ â‰¤â„¤-up x y p)

â‰¤â„¤-anti : (x y : â„¤) â†’ x â‰¤â„¤ y â†’ y â‰¤â„¤ x â†’ x â‰¡ y
â‰¤â„¤-anti (pos x) (pos y) xâ‰¤y yâ‰¤x = ap pos (â‰¤-anti x y xâ‰¤y yâ‰¤x)
â‰¤â„¤-anti (negsucc x) (negsucc y) xâ‰¤y yâ‰¤x = ap negsucc (â‰¤-anti x y yâ‰¤x xâ‰¤y)

unsucc-â‰¤â„¤ : (x y : â„¤) â†’ succâ„¤ x â‰¤â„¤ succâ„¤ y â†’ x â‰¤â„¤ y
unsucc-â‰¤â„¤ (pos x) (pos y) sxâ‰¤sy = sxâ‰¤sy
unsucc-â‰¤â„¤ (pos x) (negsucc 0) ()
unsucc-â‰¤â„¤ (pos x) (negsucc (succ y)) ()
unsucc-â‰¤â„¤ (negsucc x) (pos y) sxâ‰¤sy = â‹†
unsucc-â‰¤â„¤ (negsucc x) (negsucc 0) sxâ‰¤sy = â‹†
unsucc-â‰¤â„¤ (negsucc (succ x)) (negsucc (succ y)) sxâ‰¤sy = sxâ‰¤sy

belowâ†’below' : (x y : â„¤) â†’ x below y â†’ x below' y
belowâ†’below' x y (p , q)
 = Cases (â‰¤â„¤-split (downLeft y) x p) (inl âˆ˜ _â»Â¹)
     Î» lyâ‰¤sx â†’ Cases (â‰¤â„¤-split x (downRight y) q) (inr âˆ˜ inr)
     (Î» xâ‰¤sry â†’ inr (inl (â‰¤â„¤-anti x (downMid y) (unsucc-â‰¤â„¤ x (downMid y) xâ‰¤sry) lyâ‰¤sx)))

â‰¤â„¤-succ : (x : â„¤) â†’ x â‰¤â„¤ succâ„¤ x
â‰¤â„¤-succ (pos x) = â‰¤-succ x
â‰¤â„¤-succ (negsucc 0) = â‹†
â‰¤â„¤-succ (negsucc (succ x)) = â‰¤-succ x

â‰¤â„¤-trans : (x y z : â„¤) â†’ x â‰¤â„¤ y â†’ y â‰¤â„¤ z â†’ x â‰¤â„¤ z
â‰¤â„¤-trans (pos x) (pos y) (pos z) p q = â‰¤-trans x y z p q
â‰¤â„¤-trans (negsucc x) (negsucc y) (negsucc 0) p q = â‹†
â‰¤â„¤-trans (negsucc x) (negsucc y) (negsucc (succ z)) p q = â‰¤-trans (succ z) y x q p
â‰¤â„¤-trans (negsucc x) (pos y) (pos z) p q = â‹†
â‰¤â„¤-trans (negsucc x) (negsucc y) (pos z) p q = â‹†

â‰¤â„¤-refl : (x : â„¤) â†’ x â‰¤â„¤ x
â‰¤â„¤-refl (pos x) = â‰¤-refl x
â‰¤â„¤-refl (negsucc x) = â‰¤-refl x

below'â†’below : (x y : â„¤) â†’ x below' y â†’ x below y
below'â†’below .(downLeft y) y (inl refl)
 = â‰¤â„¤-refl (y +â„¤ y)
 , â‰¤â„¤-trans (y +â„¤ y) (succâ„¤ (y +â„¤ y)) (succâ„¤ (succâ„¤ (y +â„¤ y)))
     (â‰¤â„¤-succ (y +â„¤ y))
     (â‰¤â„¤-succ (succâ„¤ (y +â„¤ y)))
below'â†’below .(downMid y) y (inr (inl refl))
 = â‰¤â„¤-succ (y +â„¤ y)
 , â‰¤â„¤-succ (succâ„¤ (y +â„¤ y))
below'â†’below .(downRight y) y (inr (inr refl))
 = â‰¤â„¤-trans (y +â„¤ y) (succâ„¤ (y +â„¤ y)) (succâ„¤ (succâ„¤ (y +â„¤ y)))
     (â‰¤â„¤-succ (y +â„¤ y))
     (â‰¤â„¤-succ (succâ„¤ (y +â„¤ y)))
 , â‰¤â„¤-refl (succâ„¤ (succâ„¤ (y +â„¤ y)))

ğ•‚ : ğ“¤â‚€ Ì‡
ğ•‚ = Î£ Î± ê‰ (â„¤ â†’ â„¤) , Î  n ê‰ â„¤ , Î± n below Î± (predâ„¤ n) 

Ã—-decidable : {X : ğ“¤ Ì‡ } {Y : ğ“¥ Ì‡ }
            â†’ decidable X â†’ decidable Y â†’ decidable (X Ã— Y)
Ã—-decidable (inl  x) (inl  y) = inl (x , y)
Ã—-decidable (inl  _) (inr Â¬y) = inr (Î» (_ , y) â†’ Â¬y y)
Ã—-decidable (inr Â¬x) (inl  _) = inr (Î» (x , _) â†’ Â¬x x)
Ã—-decidable (inr Â¬x) (inr  _) = inr (Î» (x , _) â†’ Â¬x x)

+-decidable : {X : ğ“¤ Ì‡ } {Y : ğ“¥ Ì‡ }
            â†’ decidable X â†’ decidable Y â†’ decidable (X + Y)
+-decidable (inl  x) _        = inl (inl x)
+-decidable (inr Â¬x) (inl  y) = inl (inr y)
+-decidable (inr Â¬x) (inr Â¬y) = inr (cases Â¬x Â¬y)

â‰¤â„¤-decidable : (x y : â„¤) â†’ decidable (x â‰¤â„¤ y)
â‰¤â„¤-decidable (pos x) (pos y)         = â‰¤-decidable x y
â‰¤â„¤-decidable (negsucc x) (negsucc y) = â‰¤-decidable y x
â‰¤â„¤-decidable (pos _) (negsucc _)     = inr id
â‰¤â„¤-decidable (negsucc _) (pos _)     = inl â‹†

below-decidable : (x y : â„¤) â†’ decidable (x below y)
below-decidable x y
 = Ã—-decidable
     (â‰¤â„¤-decidable (downLeft y) x)
     (â‰¤â„¤-decidable x (downRight y))
```

Definition of share-ancestor and properties

```agda
share-ancestor : (x y : â„¤) â†’ ğ“¤â‚€ Ì‡
share-ancestor x y = Î£ z ê‰ â„¤ , (x below z) Ã— (y below z)

upRight-succ : (x : â„¤) â†’ upRight (succâ„¤ (succâ„¤ x)) â‰¡ succâ„¤ (upRight x)
upRight-succ (pos x) = refl
upRight-succ (negsucc 0) = refl
upRight-succ (negsucc 1) = refl
upRight-succ (negsucc (succ (succ x))) = refl

upLeft'-succ : (x : â„¤) â†’ (p : even x + odd x)
             â†’ upLeft (succâ„¤ (succâ„¤ x)) â‰¡ succâ„¤ (upLeft' x p)
upLeft'-succ x (inl e) = upLeft-even (succâ„¤ (succâ„¤ x)) (even-succ2 x e)
                       âˆ™ (succpredâ„¤ (upRight x)
                       âˆ™ predsuccâ„¤ (upRight x) â»Â¹
                       âˆ™ ap predâ„¤ (upRight-succ x â»Â¹)) â»Â¹
upLeft'-succ x (inr o) = upLeft-odd (succâ„¤ (succâ„¤ x)) (odd-succ2 x o)
                       âˆ™ upRight-succ x

upLeft-succ : (x : â„¤) â†’ upLeft (succâ„¤ (succâ„¤ x)) â‰¡ succâ„¤ (upLeft x)
upLeft-succ x = upLeft'-succ x (even-or-odd? x)

downLeft-below : (x : â„¤) â†’ downLeft x below x
downLeft-below x = (â‰¤â„¤-refl (x +â„¤ x))
                 , â‰¤â„¤-trans (x +â„¤ x) (succâ„¤ (x +â„¤ x)) (succâ„¤ (succâ„¤ (x +â„¤ x)))
                     (â‰¤â„¤-succ (x +â„¤ x))
                     (â‰¤â„¤-succ (succâ„¤ (x +â„¤ x)))

downMid-below : (x : â„¤) â†’ downMid x below x
downMid-below x = {!!}

downRight-below : (x : â„¤) â†’ downRight x below x
downRight-below x = {!!}

{-
x/2-double-even : (x : â„¤) â†’ even x â†’ ((x /2) +â„¤ (x /2)) â‰¡ x
x/2-double-even = ?

x/2-double-odd : (x : â„¤) â†’ odd x â†’ ((x /2) +â„¤ (x /2)) â‰¡ x +â„¤ (sign x 1)
x/2-double-odd = ?
-}

up-below-right : (x : â„¤) â†’ x below upRight x
up-below-right (pos zero) = â‹† , â‹†
up-below-right (pos (succ zero)) = â‹† , â‹†
up-below-right (pos (succ (succ x)))
 = transport (pos (succ (succ x)) below_) (upRight-succ (pos x) â»Â¹)
     (below'â†’below (pos (succ (succ x))) (pos (succ (x /2))) {!!})
up-below-right (negsucc zero) = â‹† , â‹†
up-below-right (negsucc (succ zero)) = â‹† , â‹†
up-below-right (negsucc (succ (succ x))) = {!!}

up-below : (x : â„¤) â†’ (x below upLeft x) Ã— (x below upRight x)
up-below = {!!} 

below-up : (x y : â„¤) â†’ x below y â†’ (y â‰¡ upLeft x) + (y â‰¡ upRight x)
below-up x y (p , q) = {!!}

share-ancestor-up : (x y : â„¤) â†’ share-ancestor x y
                  â†’ (upLeft  x â‰¡ upLeft y) + (upLeft  x â‰¡ upRight y)
                  + (upRight x â‰¡ upLeft y) + (upRight x â‰¡ upRight y)
share-ancestor-up x y (z , p , q) = Î³ x y z (below-up x z p) (below-up y z q) where
  Î³ : âˆ€ x y z
    â†’ (z â‰¡ upLeft x) + (z â‰¡ upRight x)
    â†’ (z â‰¡ upLeft y) + (z â‰¡ upRight y)
    â†’ (upLeft  x â‰¡ upLeft y) + (upLeft  x â‰¡ upRight y)
    + (upRight x â‰¡ upLeft y) + (upRight x â‰¡ upRight y)
  Î³ x y .(upLeft x)  (inl refl) (inl r) = inl r
  Î³ x y .(upLeft x)  (inl refl) (inr r) = inr (inl r)
  Î³ x y .(upRight x) (inr refl) (inl r) = inr (inr (inl r))
  Î³ x y .(upRight x) (inr refl) (inr r) = inr (inr (inr r))

share-ancestor-decidable : (x y : â„¤) â†’ decidable (share-ancestor x y)
share-ancestor-decidable x y = Cases Î³ (inl âˆ˜ Î´) (inr âˆ˜ Î¶)
 where
   Î³ : decidable ((y below upLeft x) + (y below upRight x)) 
   Î³ = +-decidable (below-decidable y (upLeft x)) (below-decidable y (upRight x))
   Î´ : (y below upLeft x) + (y below upRight x) â†’ share-ancestor x y
   Î´ (inl g) = upLeft  x , prâ‚ (up-below x) , g
   Î´ (inr g) = upRight x , prâ‚‚ (up-below x) , g
   Î¶ : Â¬ ((y below upLeft x) + (y below upRight x)) â†’ Â¬ share-ancestor x y
   Î¶ f (z , p , q) = f (Cases (below-up x z p)
                         (Î» l â†’ inl (transport (y below_) l q))
                         (Î» r â†’ inr (transport (y below_) r q)))

share-ancestor-refl : (x : â„¤) â†’ share-ancestor x x
share-ancestor-refl x = upRight x , prâ‚‚ (up-below x) , prâ‚‚ (up-below x)

share-ancestor-sym : (x y : â„¤) â†’ share-ancestor x y â†’ share-ancestor y x
share-ancestor-sym x y (z , p , q) = z , q , p

share-ancestor-up2 : (x : â„¤) â†’ share-ancestor (upLeft x) (upRight x)
share-ancestor-up2 x = {!!}

share-ancestor-trans : (x y z : â„¤)
                     â†’ ((a , _) : share-ancestor x y)
                     â†’ ((b , _) : share-ancestor y z)
                     â†’ share-ancestor a b
share-ancestor-trans x y z (a , p) (b , q)
 = Cases Î³ (Cases Î´ f g) (Cases Î´ h i)
 where
   Î³ : (a â‰¡ upLeft y) + (a â‰¡ upRight y)
   Î³ = below-up y a (prâ‚‚ p)
   Î´ : (b â‰¡ upLeft y) + (b â‰¡ upRight y)
   Î´ = below-up y b (prâ‚ q)
   f : b â‰¡ upLeft y â†’ a â‰¡ upLeft y â†’ share-ancestor a b
   f w e = transport (share-ancestor a) (e âˆ™ w â»Â¹)
             (share-ancestor-refl a)
   g : b â‰¡ upRight y â†’ a â‰¡ upLeft y â†’ share-ancestor a b
   g w e = transport (share-ancestor a) (w â»Â¹)
             (transport (Î» - â†’ share-ancestor - (upRight y)) (e â»Â¹)
               (share-ancestor-up2 y))
   h : b â‰¡ upLeft y â†’ a â‰¡ upRight y â†’ share-ancestor a b
   h w e = transport (share-ancestor a) (w â»Â¹)
             (transport (Î» - â†’ share-ancestor - (upLeft y)) (e â»Â¹)
               (share-ancestor-sym (upLeft y) (upRight y)
                 (share-ancestor-up2 y)))
   i : b â‰¡ upRight y â†’ a â‰¡ upRight y â†’ share-ancestor a b
   i w e = transport (share-ancestor a) (e âˆ™ w â»Â¹)
             (share-ancestor-refl a)


above-share-ancestor : (x y a b : â„¤) â†’ x below a â†’ y below b
                     â†’ ((c , _) : share-ancestor x y)
                     â†’ share-ancestor a b
above-share-ancestor x y a b p q (c , r , s)
 = share-ancestor-trans x (downMid c) y (a , p , {!!}) (b , {!!} , q)

```

Definition of closeness function for sequences

```agda
dec-to-ğŸš : {X : ğ“¤ Ì‡ } â†’ decidable X â†’ ğŸš
dec-to-ğŸš (inl _) = â‚
dec-to-ğŸš (inr _) = â‚€

dec-to-ğŸš-is-â‚ : {X : ğ“¤ Ì‡ } â†’ {d : decidable X} â†’ X â†’ dec-to-ğŸš d â‰¡ â‚
dec-to-ğŸš-is-â‚ {_} {_} {inl  _} _ = refl
dec-to-ğŸš-is-â‚ {_} {_} {inr Â¬x} x = ğŸ˜-elim (Â¬x x)

dec-to-ğŸš-was-â‚ : {X : ğ“¤ Ì‡ } â†’ {d : decidable X} â†’ dec-to-ğŸš d â‰¡ â‚ â†’ X
dec-to-ğŸš-was-â‚ {_} {_} {inl x} _ = x
dec-to-ğŸš-was-â‚ {_} {_} {inr _} z = ğŸ˜-elim (zero-is-not-one z)

c' : {Y : â„• â†’ ğ“¥ Ì‡ } â†’ (ds : (n : â„•) â†’ decidable (Y n))
   â†’ ((n : â„•) â†’ Y (succ n) â†’ Y n) â†’ â„•âˆ
c' ds f
 = (Î» n   â†’ dec-to-ğŸš (ds n))
 , (Î» n r â†’ dec-to-ğŸš-is-â‚ (f n (dec-to-ğŸš-was-â‚ r))) 
```

discrete-cc : {X : ğ“¤ Ì‡ } â†’ is-discrete X â†’ X Ã— X â†’ â„•âˆ
discrete-cc ds (x , y) = c' (Î» _ â†’ ds x y) (Î» _ â†’ id)

Definition of closeness function for ğ•‚

```agda
c : ğ•‚ Ã— ğ•‚ â†’ â„•âˆ
c  ((Î± , Î³Î±) , (Î² , Î³Î²))
 = c' (Î» n â†’ share-ancestor-decidable (Î± (pos n)) (Î² (pos n)))
      (Î» n â†’ above-share-ancestor
               (Î± (pos (succ n)))  (Î² (pos (succ n)))
               (Î± (pos       n ))  (Î² (pos       n ))
              (Î³Î± (pos (succ n))) (Î³Î² (pos (succ n))))

c-sym : (Î± Î² : ğ•‚) â†’ c (Î± , Î²) â‰¡ c (Î² , Î±)
c-sym (Î± , Î³Î±) (Î² , Î³Î²)
 = â„•âˆ-equals Î» i â†’ ?

c-eai : (Î± : ğ•‚) â†’ c (Î± , Î±) â‰¡ âˆ
c-eai (Î± , _)
 = â„•âˆ-equals (Î» i â†’ dec-to-ğŸš-is-â‚ (share-ancestor-refl (Î± (pos i))))

c-ult' : (Î± Î² Î¶ : ğ•‚) (n : â„•) â†’ prâ‚ (min (c (Î± , Î²)) (c (Î² , Î¶))) (succ n) â‰¡ â‚
       â†’ prâ‚ (c (Î± , Î¶)) n â‰¡ â‚
c-ult' Î± Î² Î¶ n r
 = {!!}

c-ult : (Î± Î² Î¶ : ğ•‚) â†’ min (c (Î± , Î²)) (c (Î² , Î¶)) â‰¼ c (Î± , Î¶)
c-ult Î± Î² Î¶ n r
 = {!prâ‚‚ (c (Î± , Î¶!}
 {- dec-to-ğŸš-is-â‚
     (share-ancestor-trans
       (prâ‚ Î± (pos n))
       (prâ‚ Î² (pos n))
       (prâ‚ Î¶ (pos n))
       (dec-to-ğŸš-was-â‚ (Lemma[minğŸšabâ‰¡â‚â†’aâ‰¡â‚] {prâ‚ (c (Î± , Î²)) n} {prâ‚ (c (Î² , Î¶)) n} r))
       (dec-to-ğŸš-was-â‚ (Lemma[minğŸšabâ‰¡â‚â†’bâ‰¡â‚] {prâ‚ (c (Î± , Î²)) n} {prâ‚ (c (Î² , Î¶)) n} r))) -}

-- Incorrect!! The sequences don't converge
c-iae : (Î± Î² : ğ•‚) â†’ c (Î± , Î²) â‰¡ âˆ â†’ Î± â‰¡ Î²
c-iae (Î± , _) (Î² , _) e = {!!}
 where
   Î³ : Î± â‰¡ Î²
   Î³ = {!!}
```
