```agda
{-# OPTIONS --without-K --exact-split #-}

open import UF-FunExt
open import SpartanMLTT

module TernaryBoehmRealsPrelude (fe : FunExt) where

open import Two-Properties hiding (zero-is-not-one)
open import NaturalsOrder
open import NaturalsAddition renaming (_+_ to _+â„•_)
open import IntegersB
open import IntegersOrder
open import IntegersAddition renaming (_+_ to _+â„¤_)
open import IntegersNegation renaming (-_  to  âˆ’â„¤_)
open import UF-Subsingletons
open import NaturalsOrder
open import DecidableAndDetachable

succ-lc : (x y : â„•) â†’ succ x â‰¡ succ y â†’ x â‰¡ y
succ-lc x x refl = refl

â„•-is-discrete : (x y : â„•) â†’ decidable (x â‰¡ y)
â„•-is-discrete zero zero = inl refl
â„•-is-discrete zero (succ y) = inr (Î» ())
â„•-is-discrete (succ x) zero = inr (Î» ())
â„•-is-discrete (succ x) (succ y)
 = Cases (â„•-is-discrete x y)
     (inl âˆ˜ ap succ)
     (inr âˆ˜ Î» f g â†’ f (succ-lc x y g))

pos-lc : (x y : â„•) â†’ pos x â‰¡ pos y â†’ x â‰¡ y
pos-lc x x refl = refl

negsucc-lc : (x y : â„•) â†’ negsucc x â‰¡ negsucc y â†’ x â‰¡ y
negsucc-lc x x refl = refl

â„¤-is-discrete : (x y : â„¤) â†’ decidable (x â‰¡ y)
â„¤-is-discrete (pos     x) (pos     y)
 = Cases (â„•-is-discrete x y)
     (inl âˆ˜ ap pos)
     (inr âˆ˜ (Î» f g â†’ f (pos-lc x y g)))
â„¤-is-discrete (negsucc x) (negsucc y)
 = Cases (â„•-is-discrete x y)
     (inl âˆ˜ ap negsucc)
     (inr âˆ˜ (Î» f g â†’ f (negsucc-lc x y g)))
â„¤-is-discrete (pos     _) (negsucc _) = inr (Î» ())
â„¤-is-discrete (negsucc _) (pos     _) = inr (Î» ())

_â‰¤â„¤_â‰¤â„¤_ : â„¤ â†’ â„¤ â†’ â„¤ â†’ ğ“¤â‚€ Ì‡ 
x â‰¤â„¤ y â‰¤â„¤ z = (x â‰¤â„¤ y) Ã— (y â‰¤â„¤ z)

â‰¤â„¤Â²-is-prop : {l u : â„¤} (x : â„¤) â†’ is-prop (l â‰¤â„¤ x â‰¤â„¤ u)
â‰¤â„¤Â²-is-prop {l} {u} x = Ã—-is-prop (â„¤â‰¤-is-prop l x) (â„¤â‰¤-is-prop x u)

data ğŸ› : ğ“¤â‚€ Ì‡ where
  âˆ’1 O +1 : ğŸ›

_/2 : â„• â†’ â„•
0 /2 = 0
1 /2 = 0
succ (succ n) /2 = succ (n /2)

sign : â„¤ â†’ (â„• â†’ â„¤)
sign (pos     _) = pos
sign (negsucc _) = negsucc

num : â„¤ â†’ â„•
num  (pos     n) = n
num  (negsucc n) = n

odd even : â„¤ â†’ ğ“¤â‚€ Ì‡
odd (pos                   0) = ğŸ˜
odd (pos                   1) = ğŸ™
odd (pos (succ (succ x)))     = odd (pos x)
odd (negsucc               0) = ğŸ™
odd (negsucc               1) = ğŸ˜
odd (negsucc (succ (succ x))) = odd (negsucc x)
even x = Â¬ odd x

even-or-odd? : (x : â„¤) â†’ even x + odd x
even-or-odd? (pos                   0) = inl (Î» x â†’ x)
even-or-odd? (pos                   1) = inr â‹†
even-or-odd? (pos (succ (succ x)))     = even-or-odd? (pos x)
even-or-odd? (negsucc               0) = inr â‹†
even-or-odd? (negsucc               1) = inl (Î» x â†’ x)
even-or-odd? (negsucc (succ (succ x))) = even-or-odd? (negsucc x)

odd-is-prop : (x : â„¤) â†’ is-prop (odd x)
odd-is-prop (pos                   0) = ğŸ˜-is-prop
odd-is-prop (pos                   1) = ğŸ™-is-prop
odd-is-prop (pos (succ (succ x)))     = odd-is-prop (pos x)
odd-is-prop (negsucc               0) = ğŸ™-is-prop
odd-is-prop (negsucc               1) = ğŸ˜-is-prop
odd-is-prop (negsucc (succ (succ x))) = odd-is-prop (negsucc x)

succ-odd-is-even : (x : â„¤) â†’ odd x â†’ even (succâ„¤ x)
succ-odd-is-even (pos                          1) o = id
succ-odd-is-even (pos            (succ (succ x))) o = succ-odd-is-even (pos x) o
succ-odd-is-even (negsucc                      0) o = id
succ-odd-is-even (negsucc (succ (succ (succ x)))) o = succ-odd-is-even (negsucc (succ x)) o

succ-even-is-odd : (x : â„¤) â†’ even x â†’ odd (succâ„¤ x)
succ-even-is-odd (pos                          0) e = â‹†
succ-even-is-odd (pos                          1) e = e â‹†
succ-even-is-odd (pos            (succ (succ x))) e = succ-even-is-odd (pos x) e
succ-even-is-odd (negsucc                      0) e = e â‹†
succ-even-is-odd (negsucc                      1) e = â‹†
succ-even-is-odd (negsucc                      2) e = e â‹†
succ-even-is-odd (negsucc (succ (succ (succ x)))) e = succ-even-is-odd (negsucc (succ x)) e

odd-succ-succ : (x : â„¤) â†’ odd x â†’ odd (succâ„¤ (succâ„¤ x))
odd-succ-succ (pos x) = id
odd-succ-succ (negsucc zero) = id
odd-succ-succ (negsucc (succ (succ x))) = id

even-succ-succ : (x : â„¤) â†’ even x â†’ even (succâ„¤ (succâ„¤ x))
even-succ-succ (pos x) = id
even-succ-succ (negsucc zero) = id
even-succ-succ (negsucc (succ (succ x))) = id

even-is-prop : (x : â„¤) â†’ is-prop (even x)
even-is-prop x p q = dfunext (fe _ _) (Î» i â†’ ğŸ˜-elim (p i))

even-or-odd-is-prop : (x : â„¤) â†’ is-prop (even x + odd x)
even-or-odd-is-prop x = +-is-prop (even-is-prop x) (odd-is-prop x) id

_âˆ’â„¤_ : â„¤ â†’ â„¤ â†’ â„¤
x âˆ’â„¤ y = x +â„¤ (âˆ’â„¤ y)

â„¤[_,_] : â„¤ â†’ â„¤ â†’ ğ“¤â‚€ Ì‡
â„¤[ l , u ] = Î£ z ê‰ â„¤ , (l â‰¤â„¤ z â‰¤â„¤ u)

â„¤[_,_]-succ : (l u : â„¤) â†’ â„¤[ l , u ] â†’ â„¤[ l , succâ„¤ u ]
â„¤[ l , u ]-succ (z , lâ‰¤z , zâ‰¤u) = z , lâ‰¤z , â„¤â‰¤-trans z u (succâ„¤ u) zâ‰¤u (1 , refl) 

â‰¤â„¤-antisym : âˆ€ x y â†’ x â‰¤â„¤ y â‰¤â„¤ x â†’ x â‰¡ y
â‰¤â„¤-antisym x y (xâ‰¤y , yâ‰¤x) with â„¤â‰¤-split x y xâ‰¤y | â„¤â‰¤-split y x yâ‰¤x
... | inl (n , Î³) | inl (m , Î´)
 = ğŸ˜-elim (â„¤-equal-not-less-than x (â„¤<-trans x y x (n , Î³) (m , Î´)))
... | inl  _  | inr yâ‰¡x = yâ‰¡x â»Â¹
... | inr xâ‰¡y | _       = xâ‰¡y

â‰¤â„¤-back : âˆ€ x y â†’ x <â„¤ y â†’ x â‰¤â„¤ predâ„¤ y
â‰¤â„¤-back x .(succâ„¤ x +â„¤ pos n) (n , refl)
 = â„¤â‰¤-trans x (x +pos n) (predâ„¤ (succâ„¤ x +pos n))
     (n , refl)
     (transport ((x +pos n) â‰¤â„¤_)
       (predsuccâ„¤ (x +pos n) â»Â¹
       âˆ™ ap predâ„¤ (â„¤-left-succ x (pos n) â»Â¹))
       (â„¤â‰¤-refl (x +pos n)))
